src/program_proof/rsm/distx/invariance/commit.v
@@ -548,6 +548,7 @@ Section inv.
         iAssert (⌜dom wrs ⊆ keys_all ∧ tid ≠ O⌝)%I as %[Hdom Htidnz].
         { iDestruct "Hprep" as "[Hwrs _]".
           iDestruct (txnwrs_lookup with "Hwrsm Hwrs") as %Hlookup.
+          apply lookup_wrsm_dbmap_Some in Hlookup.
           specialize (Hwrsm _ _ Hlookup). simpl in Hwrsm.
           destruct Hwrsm as [Hvt Hvw].
           iPureIntro.
@@ -624,6 +625,7 @@ Section inv.
         (* Obtain [correct_wrs γ tid wrs]. *)
         iDestruct "Hprep" as "[Hwrs _]".
         iDestruct (txnwrs_lookup with "Hwrsm Hwrs") as %Hwrs.
+        apply lookup_wrsm_dbmap_Some in Hwrs.
         iDestruct (big_sepM_lookup with "Hcwrs") as "Hpos"; first apply Hwrs.
         iDestruct (correct_incorrect_wrs with "Hpos Hneg") as %[].
       }
@@ -646,6 +648,7 @@ Section inv.
     iAssert (⌜dom wrs ⊆ keys_all⌝)%I as %Hdom.
     { iDestruct "Hprep" as "[Hwrs _]".
       iDestruct (txnwrs_lookup with "Hwrsm Hwrs") as %Hlookup.
+      apply lookup_wrsm_dbmap_Some in Hlookup.
       specialize (Hwrsm _ _ Hlookup).
       by destruct Hwrsm as [_ Hgoal].
     }
